lot's of different stuff

theories/lam/lib/fixlam.v
@@ -28,77 +28,137 @@ Qed.
 Lemma FixArrow_eval f : nsteps lam_step 2 (FixArrow f) (f (Lam ((FixArrow f).[ren (+1)] %0)))%Eₙₒ.
 Proof. do 2 (eapply nsteps_l; first auto_lam_step; asimpl). by apply nsteps_O. Qed.
 
-Definition FixLamBodyHelp (e : expr) := Lam ((Lam (e.[(%0 ())%Eₙₒ .: ren (+1)].[ren (+1)]))).
+Definition Rec (e : {bind 2 of expr}) : val :=
+  LamV ((FixArrow (Lam (Lam e))).[ren (+1)] %0)%Eₙₒ.
 
-Definition FixLam (e : expr) :=
-  (Lam ((FixArrow (FixLamBodyHelp e)).[ren (+1)] %0) ())%Eₙₒ.
+(* Definition Rec (e : {bind 2 of expr}) : expr := *)
+(*   Lam ((FixArrow (Lam (Lam e.[upn 0 (ren (lookup_n (swap_list 1 1)))]))).[ren (+1)] %0)%Eₙₒ. *)
 
-Lemma FixLam_eval e : nsteps lam_step 5 (FixLam e) (e.[FixLam e/]).
+Lemma Rec_typed Γ e τ1 τ2 : (τ1 :: TArrow τ1 τ2 :: Γ ⊢ₙₒ e : τ2)
+  -> (Γ ⊢ₙₒ Rec e : TArrow τ1 τ2).
 Proof.
-  eapply nsteps_l. apply head_prim_step. auto_head_step.
-  cut (nsteps lam_step 4 ((FixArrow (FixLamBodyHelp e)) ()) e.[FixLam e/])%Eₙₒ. asimpl.
-  rewrite /FixArrow. by asimpl.
-  assert (4 = (2 + 2)%nat) as ->. done.
-  eapply nsteps_trans.
-  eapply (nsteps_congruence (fill [AppLCtx ()%Eₙₒ])). intros. apply lam_step_ctx. apply ectx_lang_ctx. apply H.
-  apply FixArrow_eval.
-  eapply nsteps_l. auto_lam_step. asimpl.
-  eapply nsteps_l. auto_lam_step. asimpl.
-  rewrite /FixLam /FixLamBodyHelp. asimpl. apply nsteps_O.
+  constructor. apply App_typed with (τ1 := τ1). apply context_weakening1. apply FixArrow_typed. constructor. by constructor. by constructor.
+  (* cut ([] ++ [τ1] ++ [TArrow τ1 τ2] ++ Γ ⊢ₙₒ e.[upn (length ([] : list type)) (ren (lookup_n (swap_list (length [τ1]) (length [TArrow τ1 τ2]))))] : τ2). by asimpl. *)
+  (* apply context_swap_typed. by simpl. by constructor. *)
 Qed.
 
-Lemma small_help Γ e τ i :
-  Γ ⊢ₙₒ e : τ → (alter (fun τ => TArrow TUnit τ) i Γ) ⊢ₙₒ e.[upn i ((%0 ())%Eₙₒ .: ren (+1))] : τ.
-Proof.
-  generalize dependent i.
-  generalize dependent τ.
-  generalize dependent Γ.
-  induction e; intros; simpl.
-  - destruct (iter_up_cases x i ((%0)%Eₙₒ ()%Eₙₒ .: ren (+1))) as [[-> lt] | [j [-> ->]]].
-    + inversion_clear H. constructor. rewrite list_lookup_alter_ne. auto. lia.
-    + inversion_clear H. destruct j. asimpl.
-      econstructor. econstructor. rewrite list_lookup_alter.
-      assert ((i + 0)%nat = i) as eq. lia. rewrite eq in H0.
-      by simplify_option_eq.
-      econstructor.
-      asimpl. constructor. rewrite list_lookup_alter_ne.
-      assert ((i + S j)%nat = S (i + j)%nat) as eq. lia. by rewrite eq in H0. lia.
-  - simpl. inversion_clear H. econstructor. eapply (IHe0 (τ1 :: Γ) τ (S i) H0). by eapply IHe.
-  - simpl. inversion_clear H. econstructor. eapply (IHe (τ1 :: Γ) τ2 (S i) H0).
-  - simpl. inversion_clear H. econstructor. by eapply IHe1. by eapply IHe2.
-  - simpl. inversion_clear H; econstructor.
-  - simpl. inversion_clear H. econstructor. by eapply IHe1. by eapply IHe2.
-  - simpl. inversion_clear H. econstructor. by eapply IHe1. by eapply IHe2. by eapply IHe3.
-  - simpl. inversion_clear H. econstructor. by eapply IHe1. by eapply IHe2.
-  - simpl. inversion_clear H. econstructor. by eapply IHe1. by eapply IHe2.
-  - simpl. inversion_clear H. econstructor. by eapply IHe.
-  - simpl. inversion_clear H. econstructor. by eapply IHe.
-  - simpl. inversion_clear H. econstructor. by eapply IHe.
-  - simpl. inversion_clear H. econstructor. by eapply IHe.
-  - simpl. inversion_clear H. econstructor. by eapply IHe.
-      by eapply (IHe0 (τ1 :: Γ) τ (S i)).
-      by eapply (IHe1 (τ2 :: Γ) τ (S i)).
-  - simpl. inversion_clear H. econstructor. by eapply IHe.
-  - simpl. inversion_clear H. econstructor. by eapply IHe.
-Qed.
-
-Lemma FixLamBodyHelp_typed Γ e τ : τ :: Γ ⊢ₙₒ e : τ → Γ ⊢ₙₒ FixLamBodyHelp e : ((TUnit ⟶ τ) ⟶ TUnit ⟶ τ)%Tₙₒ.
-Proof.
-  intro H.
-  apply Lam_typed. apply Lam_typed. change ([TUnit] ++ TUnit ⟶ τ :: Γ ⊢ₙₒ e.[%0 () .: ren (+1)].[ren (+1)] : τ). apply context_weakening.
-  cut ((alter (fun τ => TArrow TUnit τ) 0 (τ :: Γ)) ⊢ₙₒ e.[upn 0 ((%0 ())%Eₙₒ .: ren (+1))] : τ). by asimpl. by apply small_help.
-Qed.
-
-Lemma FixLam_typed Γ e τ : τ :: Γ ⊢ₙₒ e : τ → Γ ⊢ₙₒ FixLam e : τ.
-Proof.
-  intro H. apply App_typed with (τ1 := TUnit).
-  apply Lam_typed. apply App_typed with (τ1 := TUnit).
-  change ([TUnit] ++ Γ ⊢ₙₒ (FixArrow (FixLamBodyHelp e)).[ren (+1)] : TArrow TUnit τ). apply context_weakening.
-  apply FixArrow_typed. apply FixLamBodyHelp_typed. auto. by econstructor. constructor.
-Qed.
-
-Lemma FixLam_subst e σ : (FixLam e).[σ] = FixLam e.[up σ].
-Proof. rewrite /FixLam. by asimpl. Qed.
-
-Global Opaque FixLam.
 Global Opaque FixArrow.
+
+
+Lemma Rec_subst (e : {bind 2 of expr}) σ : (of_val $ Rec e).[σ] = of_val $ Rec (e.[ids 0 .: ids 1 .: σ >> ren (+2)]).
+Proof.
+  asimpl. rewrite !FixArrow_subst. by asimpl.
+Qed.
+
+Lemma App_Rec_nsteps e1 e2 v2 :
+   to_val e2 = Some v2 →
+   nsteps lam_step 5 (App (Rec e1) e2) e1.[e2, (of_val $ Rec e1)/].
+Proof.
+  intros.
+  eapply nsteps_l. auto_lam_step. simplify_custom.
+  change 4 with (2 + 2)%nat.
+  eapply nsteps_trans. apply (nsteps_lam_step_ctx (fill_item (AppLCtx _))). apply FixArrow_eval.
+  rewrite FixArrow_subst. asimpl.
+  eapply nsteps_l. auto_lam_step. simplify_custom.
+  rewrite FixArrow_subst. asimpl.
+  eapply nsteps_l. auto_lam_step. simplify_custom.
+  rewrite FixArrow_subst. asimpl.
+  rewrite (of_to_val _ _ H) /Rec.
+  apply nsteps_O.
+Qed.
+
+Global Opaque Rec.
+
+(* Lemma App_Rec_nsteps e1 e2 v2 : *)
+(*    to_val e2 = Some v2 → *)
+(*    nsteps lam_step 5 (App (Rec e1) e2) e1.[(Rec e1), e2/]. *)
+(* Proof. *)
+(*   intros. *)
+(*   eapply nsteps_l. auto_lam_step. simplify_custom. *)
+(*   change 4 with (2 + 2)%nat. *)
+(*   eapply nsteps_trans. apply (nsteps_lam_step_ctx (fill_item (AppLCtx _))). apply FixArrow_eval. *)
+(*   rewrite FixArrow_subst. asimpl. *)
+(*   eapply nsteps_l. auto_lam_step. simplify_custom. *)
+(*   rewrite FixArrow_subst. asimpl. *)
+(*   eapply nsteps_l. auto_lam_step. simplify_custom. *)
+(*   rewrite FixArrow_subst. asimpl. *)
+
+(* Lemma FixArrow_eval f : nsteps lam_step 2 (FixArrow f) (f (Lam ((FixArrow f).[ren (+1)] %0)))%Eₙₒ. *)
+(* Proof. do 2 (eapply nsteps_l; first auto_lam_step; asimpl). by apply nsteps_O. Qed. *)
+
+
+
+(* Definition FixLamBodyHelp (e : expr) := Lam ((Lam (e.[(%0 ())%Eₙₒ .: ren (+1)].[ren (+1)]))). *)
+
+(* Definition FixLam (e : expr) := *)
+(*   (Lam ((FixArrow (FixLamBodyHelp e)).[ren (+1)] %0) ())%Eₙₒ. *)
+
+(* Lemma FixLam_eval e : nsteps lam_step 5 (FixLam e) (e.[FixLam e/]). *)
+(* Proof. *)
+(*   eapply nsteps_l. apply head_prim_step. auto_head_step. *)
+(*   cut (nsteps lam_step 4 ((FixArrow (FixLamBodyHelp e)) ()) e.[FixLam e/])%Eₙₒ. asimpl. *)
+(*   rewrite /FixArrow. by asimpl. *)
+(*   assert (4 = (2 + 2)%nat) as ->. done. *)
+(*   eapply nsteps_trans. *)
+(*   eapply (nsteps_congruence (fill [AppLCtx ()%Eₙₒ])). intros. apply lam_step_ctx. apply ectx_lang_ctx. apply H. *)
+(*   apply FixArrow_eval. *)
+(*   eapply nsteps_l. auto_lam_step. asimpl. *)
+(*   eapply nsteps_l. auto_lam_step. asimpl. *)
+(*   rewrite /FixLam /FixLamBodyHelp. asimpl. apply nsteps_O. *)
+(* Qed. *)
+
+(* Lemma small_help Γ e τ i : *)
+(*   Γ ⊢ₙₒ e : τ → (alter (fun τ => TArrow TUnit τ) i Γ) ⊢ₙₒ e.[upn i ((%0 ())%Eₙₒ .: ren (+1))] : τ. *)
+(* Proof. *)
+(*   generalize dependent i. *)
+(*   generalize dependent τ. *)
+(*   generalize dependent Γ. *)
+(*   induction e; intros; simpl. *)
+(*   - destruct (iter_up_cases x i ((%0)%Eₙₒ ()%Eₙₒ .: ren (+1))) as [[-> lt] | [j [-> ->]]]. *)
+(*     + inversion_clear H. constructor. rewrite list_lookup_alter_ne. auto. lia. *)
+(*     + inversion_clear H. destruct j. asimpl. *)
+(*       econstructor. econstructor. rewrite list_lookup_alter. *)
+(*       assert ((i + 0)%nat = i) as eq. lia. rewrite eq in H0. *)
+(*       by simplify_option_eq. *)
+(*       econstructor. *)
+(*       asimpl. constructor. rewrite list_lookup_alter_ne. *)
+(*       assert ((i + S j)%nat = S (i + j)%nat) as eq. lia. by rewrite eq in H0. lia. *)
+(*   - simpl. inversion_clear H. econstructor. eapply (IHe0 (τ1 :: Γ) τ (S i) H0). by eapply IHe. *)
+(*   - simpl. inversion_clear H. econstructor. eapply (IHe (τ1 :: Γ) τ2 (S i) H0). *)
+(*   - simpl. inversion_clear H. econstructor. by eapply IHe1. by eapply IHe2. *)
+(*   - simpl. inversion_clear H; econstructor. *)
+(*   - simpl. inversion_clear H. econstructor. by eapply IHe1. by eapply IHe2. *)
+(*   - simpl. inversion_clear H. econstructor. by eapply IHe1. by eapply IHe2. by eapply IHe3. *)
+(*   - simpl. inversion_clear H. econstructor. by eapply IHe1. by eapply IHe2. *)
+(*   - simpl. inversion_clear H. econstructor. by eapply IHe1. by eapply IHe2. *)
+(*   - simpl. inversion_clear H. econstructor. by eapply IHe. *)
+(*   - simpl. inversion_clear H. econstructor. by eapply IHe. *)
+(*   - simpl. inversion_clear H. econstructor. by eapply IHe. *)
+(*   - simpl. inversion_clear H. econstructor. by eapply IHe. *)
+(*   - simpl. inversion_clear H. econstructor. by eapply IHe. *)
+(*       by eapply (IHe0 (τ1 :: Γ) τ (S i)). *)
+(*       by eapply (IHe1 (τ2 :: Γ) τ (S i)). *)
+(*   - simpl. inversion_clear H. econstructor. by eapply IHe. *)
+(*   - simpl. inversion_clear H. econstructor. by eapply IHe. *)
+(* Qed. *)
+
+(* Lemma FixLamBodyHelp_typed Γ e τ : τ :: Γ ⊢ₙₒ e : τ → Γ ⊢ₙₒ FixLamBodyHelp e : ((TUnit ⟶ τ) ⟶ TUnit ⟶ τ)%Tₙₒ. *)
+(* Proof. *)
+(*   intro H. *)
+(*   apply Lam_typed. apply Lam_typed. change ([TUnit] ++ TUnit ⟶ τ :: Γ ⊢ₙₒ e.[%0 () .: ren (+1)].[ren (+1)] : τ). apply context_weakening. *)
+(*   cut ((alter (fun τ => TArrow TUnit τ) 0 (τ :: Γ)) ⊢ₙₒ e.[upn 0 ((%0 ())%Eₙₒ .: ren (+1))] : τ). by asimpl. by apply small_help. *)
+(* Qed. *)
+
+(* Lemma FixLam_typed Γ e τ : τ :: Γ ⊢ₙₒ e : τ → Γ ⊢ₙₒ FixLam e : τ. *)
+(* Proof. *)
+(*   intro H. apply App_typed with (τ1 := TUnit). *)
+(*   apply Lam_typed. apply App_typed with (τ1 := TUnit). *)
+(*   change ([TUnit] ++ Γ ⊢ₙₒ (FixArrow (FixLamBodyHelp e)).[ren (+1)] : TArrow TUnit τ). apply context_weakening. *)
+(*   apply FixArrow_typed. apply FixLamBodyHelp_typed. auto. by econstructor. constructor. *)
+(* Qed. *)
+
+(* Lemma FixLam_subst e σ : (FixLam e).[σ] = FixLam e.[up σ]. *)
+(* Proof. rewrite /FixLam. by asimpl. Qed. *)
+
+(* Global Opaque FixLam. *)
+(* Global Opaque FixArrow. *)
