theories/prelude/big_op_three.v
@@ -10,11 +10,87 @@ Fixpoint big_sepL3 {PROP : bi} {A B C}
   | _, _,_ => False
   end%I.
 
+(* From iris Require Import bi.big_op. *)
+(* From stdpp Require Import countable fin_sets functions. *)
+(* From iris.algebra Require Export big_op. *)
+(* From iris.algebra Require Import list gmap. *)
+(* From iris.bi Require Import derived_laws_later. *)
+(* From iris.prelude Require Import options. *)
+(* Import interface.bi derived_laws.bi derived_laws_later.bi. *)
+
+
+Section big_sepL3_alt.
+
+  Context `{Σ : !gFunctors}.
+  Context {A B C : Type}.
+
+
+  Definition big_sepL3_alt
+      (Φ : A → B → C → iProp Σ) (l1 : list A) (l2 : list B) (l3 : list C) : iProp Σ :=
+    (⌜ length l1 = length l2 ⌝)%I ∧ big_sepL2 (fun _ ab c => Φ ab.1 ab.2 c) (zip l1 l2) l3.
+
+  Lemma Forall3_same_length (l : list A) (k : list B) (m : list C) :
+    Forall3 (λ _ _ _, True) l k m ↔ length l = length k ∧ length k = length m.
+  Proof.
+    split.
+    - induction 1.
+      + auto.
+      + simpl. lia.
+    - revert k m. induction l.
+      + intros ?? [? ?]. rewrite -H in H0. simpl in *.
+        destruct k, m; simpl in *; try by exfalso. constructor.
+      + intros ?? [? ?]. rewrite -H in H0. simpl in *.
+        destruct k, m; simpl in *; try by exfalso. constructor; first auto.
+        apply IHl; lia.
+  Qed.
+
+  Lemma big_sepL3_alt_equiv
+      (Φ : A → B → C → iProp Σ) (l1 : list A) (l2 : list B) (l3 : list C) :
+    big_sepL3 Φ l1 l2 l3 ⊣⊢ big_sepL3_alt Φ l1 l2 l3.
+  Proof.
+    rewrite /big_sepL3_alt.
+    apply (anti_symm _).
+    - apply bi.and_intro.
+      + revert l2 l3. induction l1 as [|x1 l1 IH]=> -[|x2 l2] -[|x3 l3] /=; auto.
+        iIntros "[H1 H2]". iDestruct (IH with "H2") as %eq. iPureIntro. lia.
+      + revert l2 l3. induction l1 as [|x1 l1 IH]=> -[|x2 l2] -[|x3 l3] /=; auto.
+        iIntros "[H1 H2]". iFrame "H1". by iApply IH.
+    - apply bi.pure_elim_l. intro eq1.
+      iIntros "H". iDestruct (big_sepL2_length with "H") as %eq2.
+      assert (Hl : Forall3 (fun _ _ _ => True) l1 l2 l3).
+      { apply Forall3_same_length. split; auto.
+        rewrite -eq2.
+        rewrite -(fmap_length snd).
+        rewrite snd_zip; auto. lia.
+      }
+      iInduction Hl as [|x1 x2 x3 l1 l2 l3 aa bb cc] "IH"; auto.
+      simpl. iDestruct "H" as "[H1 H2]". iFrame "H1".
+      simpl in *.
+      assert (eq1' : length l1 = length l2); first lia.
+      assert (eq2' : length (zip l1 l2) = length l3); first lia.
+      iSpecialize ("IH" $! eq1' eq2').
+      iApply ("IH" with "H2").
+  Qed.
+
+End big_sepL3_alt.
+
 Section big_sepL3_lemmas.
 
   Context `{Σ : !gFunctors}.
+  Context {A B C : Type}.
 
-  Lemma big_sepL3_lookup {A B C}
+  Global Instance big_sepL3_nil_persistent (Φ : A → B → C → iProp Σ) :
+    Persistent (big_sepL3 Φ [] [] []).
+  Proof. simpl; apply _. Qed.
+  Global Instance big_sepL3_persistent (Φ : A → B → C → iProp Σ) l1 l2 l3 :
+    (∀ x1 x2 x3, Persistent (Φ x1 x2 x3)) →
+    Persistent (big_sepL3 Φ l1 l2 l3).
+  Proof.
+    rewrite big_sepL3_alt_equiv /big_sepL3_alt. apply _.
+  Qed.
+
+  (* TODO; clean up versions using alt version *)
+  Lemma big_sepL3_lookup
       (Φ : A → B → C → iProp Σ) l1 l2 l3 i x1 x2 x3 :
     l1 !! i = Some x1 → l2 !! i = Some x2 → l3 !! i = Some x3 →
     big_sepL3 Φ l1 l2 l3 ⊢ Φ x1 x2 x3.
@@ -33,7 +109,7 @@ Section big_sepL3_lemmas.
       simpl. iDestruct "H" as "[a b]". auto.
   Qed.
 
-  Lemma big_sepL3_length {A B C}
+  Lemma big_sepL3_length
       (Φ : A → B → C → iProp Σ) l1 l2 l3 : big_sepL3 Φ l1 l2 l3 ⊢ ⌜ length l1 = length l2 ⌝ ∧ ⌜ length l2 = length l3 ⌝.
   Proof.
     generalize dependent l3.
@@ -44,5 +120,43 @@ Section big_sepL3_lemmas.
     - intros. destruct l2; destruct l3; auto.
       iIntros "H". simpl. rewrite IHl1. iDestruct "H" as "[H %I]". iPureIntro. lia.
   Qed.
+
+  Lemma big_sepL3_fmap_l {A' : Type} (f : A → A') (Φ : A' → B → C → iProp Σ) l1 l2 l3 :
+    big_sepL3 (fun a b c => Φ (f a) b c) l1 l2 l3
+    ⊣⊢ big_sepL3 (fun a b c => Φ a b c) (f <$> l1) l2 l3.
+  Proof.
+    generalize dependent l3.
+    generalize dependent l2.
+    generalize dependent l1.
+    induction l1.
+    - intros. destruct l2; destruct l3; auto.
+    - intros. destruct l2; destruct l3; auto. simpl. specialize (IHl1 l2 l3).
+      iSplit; iIntros "[H1 H2]"; iFrame "H1"; by iApply IHl1.
+  Qed.
+
+  Lemma big_sepL3_impl (Φ Ψ : A → B → C → iProp Σ) l1 l2 l3 :
+    ⊢ big_sepL3 Φ l1 l2 l3 -∗ □ (∀ x1 x2 x3, Φ x1 x2 x3 -∗ Ψ x1 x2 x3) -∗ big_sepL3 Ψ l1 l2 l3.
+  Proof.
+    generalize dependent l3.
+    generalize dependent l2.
+    generalize dependent l1.
+    induction l1.
+    - intros. destruct l2; destruct l3; auto.
+    - intros. destruct l2; destruct l3; auto. simpl. specialize (IHl1 l2 l3).
+      iIntros "[Habc Hl1l2l3] #Himpl". iSplitL "Habc". by iApply "Himpl". by iApply (IHl1 with "Hl1l2l3").
+  Qed.
+
+  (* Lemma big_sepL3_impl (Φ Ψ : A → B → C → iProp Σ) l1 l2 l3 : *)
+  (*   ⊢ □ (∀ x1 x2 x3, Φ x1 x2 x3 ∗-∗ Ψ x1 x2 x3) -∗ big_sepL3 Φ l1 l2 l3 ∗-∗ big_sepL3 Ψ l1 l2 l3. *)
+  (* Proof. *)
+  (*   generalize dependent l3. *)
+  (*   generalize dependent l2. *)
+  (*   generalize dependent l1. *)
+  (*   induction l1. *)
+  (*   - intros. destruct l2; destruct l3; auto. *)
+  (*   - intros. destruct l2; destruct l3; auto. simpl. specialize (IHl1 l2 l3). *)
+  (*     iIntros "#HΦΨ". *)
+  (*     iSplit; iIntros "[H1 H2]"; iSplitL "H1 HΦΨ"; try iApply "HΦΨ"; auto; try by iApply IHl1. *)
+  (* Qed. *)
 
 End big_sepL3_lemmas.
