theories/backtranslations/st_sem/expressions.v
@@ -1,0 +1,37 @@
+From st.lamst Require Import lang.
+From st.lam Require Import lang.
+From st.backtranslations.st_sem Require Import heap.
+
+Reserved Notation "<< e >>" (at level 4, e at next level).
+Fixpoint back_expr (e : lamst.lang.expr) : expr :=
+  match e with
+  | lamst.lang.Var x => Var x
+  | lamst.lang.LetIn e1 e2 => LetIn <<e1>> <<e2>>
+  | lamst.lang.Lam e => Lam <<e>>
+  | lamst.lang.App e1 e2 => App <<e1>> <<e2>>
+  | lamst.lang.Lit l => match l with
+                       | lamst.lang.LitInt n => n
+                       | lamst.lang.LitBool b => b
+                       | lamst.lang.LitUnit => LitUnit
+                       | LitLoc l => ()%Eₙₒ (* we only care about surface lang *)
+                       end
+  | lamst.lang.BinOp op e1 e2 => BinOp op <<e1>> <<e2>>
+  | lamst.lang.If e0 e1 e2 => If <<e0>> <<e1>> <<e2>>
+  | lamst.lang.Seq e1 e2 => Seq <<e1>> <<e2>>
+  | lamst.lang.Pair e1 e2 => Pair <<e1>> <<e2>>
+  | lamst.lang.Fst e => Fst <<e>>
+  | lamst.lang.Snd e => Snd <<e>>
+  | lamst.lang.InjL e => InjL <<e>>
+  | lamst.lang.InjR e => InjR <<e>>
+  | lamst.lang.Case e0 e1 e2 => Case <<e0>> <<e1>> <<e2>>
+  | lamst.lang.Fold e => Fold <<e>>
+  | lamst.lang.Unfold e => Unfold <<e>>
+  | Return e => retrn <<e>>
+  | Bind e1 e2 => bind <<e1>> <<e2>>
+  | RunST e => runst <<e>>
+  | Alloc e => alloc <<e>>
+  | Read e => read <<e>>
+  | Write e1 e2 => write <<e1>> <<e2>>
+  | Compare e1 e2 => (<<e1>> = <<e2>>)%Eₙₒ
+  end
+where "<< e >>" := (back_expr e).
