theories/backtranslations/st_sem/ghost.v
@@ -1,0 +1,48 @@
+From st.lam Require Import lang tactics lib.fixlam.
+From iris.base_logic.lib Require Export ghost_map.
+From iris.proofmode Require Import tactics.
+Require Export st.backtranslations.st_sem.list_gmap.
+
+Section ghost.
+
+  Context `{Σ : !gFunctors}.
+  Context `{irisG_inst : !irisG lam_lang Σ}.
+  Context `{ghost_mapG_inst : !ghost_mapG Σ nat V}.
+
+  Definition auth_list (γ : gname) (vs : list V) : iProp Σ :=
+    ghost_map_auth γ 1 (list_gmap vs).
+
+  Definition frag_elem (γ : gname) (i : nat) (v : V) : iProp Σ :=
+    i ↪[ γ ] v. (* ghost_map_elem γ i (DfracOwn 1) v. *)
+
+  Lemma ghost_empty :
+    ⊢ |==> ∃ γ, auth_list γ [].
+  Proof. by iApply ghost_map_alloc_empty. Qed.
+
+  Lemma ghost_alloc γ vs v :
+    auth_list γ vs -∗ |==> auth_list γ (vs ++ [v]) ∗ length vs ↪[ γ ] v.
+  Proof.
+    iIntros "Hvs".
+    rewrite !/auth_list list_gmap_snoc.
+    iApply (ghost_map_insert with "Hvs").
+    rewrite -list_gmap_lookup. by apply lookup_ge_None.
+  Qed.
+
+  Lemma ghost_write γ vs v i (Hi : vs !! i = Some v) v' :
+    auth_list γ vs ∗ i ↪[ γ ] v -∗ |==> auth_list γ (<[ i := v' ]> vs) ∗ i ↪[ γ ] v'.
+  Proof.
+    iIntros "[Hvs Hiv]".
+    rewrite !/auth_list (list_gmap_insert _ _ _ _ Hi).
+    iApply (ghost_map_update with "Hvs Hiv").
+  Qed.
+
+  Lemma ghost_read γ vs i v :
+    auth_list γ vs ∗ i ↪[ γ ] v -∗ ⌜ vs !! i = Some v ⌝.
+  Proof.
+    iIntros "[Hvs Hiv]".
+    rewrite /auth_list list_gmap_lookup.
+    iApply (ghost_map_lookup with "Hvs Hiv").
+  Qed.
+
+End ghost.
+
