theories/backtranslations/st_sem/list_gmap.v
@@ -1,0 +1,46 @@
+From st.lam Require Import lang tactics lib.fixlam.
+From iris.base_logic.lib Require Import ghost_map.
+From iris.proofmode Require Import tactics.
+
+Section list_gmap.
+
+  Context {V : Type}.
+
+  Definition list_gmap (ls : list V) : gmap nat V := map_seq 0 ls.
+
+  Lemma list_gmap_lookup ls i : ls !! i = list_gmap ls !! i.
+  Proof. rewrite /list_gmap. by rewrite lookup_map_seq_0. Qed.
+
+  Lemma list_gmap_snoc ls l : list_gmap (ls ++ [l]) = <[ length ls := l ]> (list_gmap ls).
+  Proof. by rewrite /list_gmap map_seq_snoc. Qed.
+
+  Lemma list_gmap_insert ls l l' i (H : ls !! i = Some l) :
+    list_gmap (<[i := l']> ls) = <[i := l']> (list_gmap ls).
+  Proof.
+    rewrite /list_gmap.
+    rewrite -(take_drop_middle ls i l H).
+    (* rewrite left side *)
+    assert (i < length ls). by eapply lookup_lt_Some.
+    assert (i = length (take i ls) + 0).
+    { rewrite take_length_le; lia. }
+    assert (map_seq 0 (<[i:=l']> (take i ls ++ l :: drop (S i) ls)) =
+            map_seq 0 (<[(length (take i ls) + 0):=l']> (take i ls ++ l :: drop (S i) ls))
+           ) as ->. by rewrite -H1.
+    rewrite insert_app_r. simpl.
+    (* both sides *)
+    rewrite !map_seq_app.
+    (* right side *)
+    rewrite insert_union_r. 2: rewrite lookup_map_seq_0; apply lookup_take_ge; lia.
+    (* simpl *)
+    rewrite take_length_le; try by lia. change (0 + i) with i.
+    (* both sides *)
+    change (l' :: drop (S i) ls) with ([l'] ++ drop (S i) ls).
+    change (l :: drop (S i) ls) with ([l] ++ drop (S i) ls).
+    rewrite !map_seq_app.
+    simpl.
+    (* rigth side *)
+    rewrite insert_union_l !insert_empty insert_singleton.
+    done.
+  Qed.
+
+End list_gmap.
