theories/backtranslations/st_sem/well_defined/logrel/definition.v
@@ -1,0 +1,175 @@
+From iris Require Import program_logic.weakestpre.
+From iris.proofmode Require Import tactics.
+From st.lamst Require Import types.
+From st.lam Require Import lang wkpre generic.lift.
+From iris.base_logic.lib Require Import invariants.
+From st.backtranslations.st_sem Require Import ghost heap.
+From st.prelude Require Import big_op_three.
+
+Canonical Structure typeO := leibnizO type. (* indexed by ST types *)
+
+Section value_relation.
+
+  Context `{Σ : !gFunctors}.
+  Context `{irisG_inst : !irisG lam_lang Σ}.
+  Context `{ghost_mapG_inst : !ghost_mapG Σ nat (prod val val)}.
+
+  Context (Δ : list gname).
+
+  Fixpoint valrel_typed_gen_pre (Ψ : typeO -n> valO -n> valO -n> iPropO Σ) (τ : typeO) : valO -n> valO -n> iPropO Σ := λne v v',
+    (match τ with
+     | TUnit => ⌜ v = (()%Vₙₒ : valO) ⌝ ∧ ⌜ v' = (()%Vₙₒ : valO) ⌝
+     | TBool => ∃ b : bool, ⌜ v = b ⌝ ∧ ⌜ v' = b ⌝
+     | TInt => ∃ z : Z, ⌜ v = z ⌝ ∧ ⌜ v' = z ⌝
+     | TProd τ1 τ2 => ∃ v1 v2 v1' v2', ⌜ v = (v1, v2)%Vₙₒ ⌝ ∧ ⌜ v' = (v1' , v2')%Vₙₒ ⌝ ∗ valrel_typed_gen_pre Ψ τ1 v1 v1' ∗ valrel_typed_gen_pre Ψ τ2 v2 v2'
+     | TSum τ1 τ2 => ∃ vi vi', (⌜ v = InjLV vi ⌝ ∧ ⌜ v' = InjLV vi' ⌝ ∧ valrel_typed_gen_pre Ψ τ1 vi vi') ∨
+                              (⌜ v = InjRV vi ⌝ ∧ ⌜ v' = InjRV vi' ⌝ ∧ valrel_typed_gen_pre Ψ τ2 vi vi')
+     | TArrow τ1 τ2 => □ (∀ w w', valrel_typed_gen_pre Ψ τ1 w w' -∗ lift NotStuck (valrel_typed_gen_pre Ψ τ2) (v w) (v' w'))
+     | TRec τb => ∃ w w', ⌜ v = FoldV w ⌝ ∧ ⌜ v' = FoldV w' ⌝ ∧ ▷ (Ψ τb.[TRec τb/] w w')
+     | TVar X => False
+     | TSTref ρ τ =>
+       match ρ with
+       | TVar X =>
+         match Δ !! X with
+         | Some γ => ∃ i : nat, ⌜ v = i ⌝ ∧ ⌜ v' = i ⌝ ∧
+                             inv (nroot .@ γ .@ i) (∃ (w w' : val), i ↪[γ] (w,w') ∗ valrel_typed_gen_pre Ψ τ w w')
+         | None => False
+         end
+       | _ => False
+       end
+     | TST ρ τ' =>
+       match ρ with
+       | TVar X =>
+         match Δ !! X with
+         | Some γ => ∀ psᵢ : list (prod val val),
+             let vs := psᵢ.*1 in
+             let vs' := psᵢ.*2 in
+             □ (auth_list γ psᵢ -∗
+                          WP v (encode vs) {{ x, ∃ (w w' : val) (psₜ : list (prod val val)), auth_list γ psₜ ∧
+                                                let ws := psₜ.*1 in
+                                                let ws' := psₜ.*2 in
+                                                ⌜ x = (encode ws, w)%Vₙₒ ⌝ ∧
+                                                ⌜ rtc lam_step (v' (encode vs')) (encode ws', w')%Vₙₒ ⌝ ∧
+                                                valrel_typed_gen_pre Ψ τ' w w'
+                                           }}
+               )
+         | None => True
+         end
+       | _ => True
+       end
+     end)%I.
+
+  Definition valrel_typed_gen (Ψ : typeO -n> valO -n> valO -n> iPropO Σ) : typeO -n> valO -n> valO -n> iPropO Σ := λne τ v v', valrel_typed_gen_pre Ψ τ v v'.
+
+  Instance valrel_typed_gen_contractive : Contractive valrel_typed_gen.
+  Proof.
+    intros n P1 P2 dl. rewrite /valrel_typed_gen. intro τ. simpl.
+    induction τ; try by solve_contractive.
+    - intros v v'. simpl. do 6 f_equiv. specialize (IHτ1 a a0). simpl in IHτ1. by rewrite IHτ1.
+      rewrite /lift. do 5 f_equiv. specialize (IHτ2 a1 a2). simpl in IHτ2. by rewrite IHτ2.
+    - intros v v'. simpl. destruct τ1; try done. clear IHτ1.
+      destruct (Δ !! X) as [γ|] eqn:eq; auto.
+      f_equiv. intros i. f_equiv. f_equiv. f_equiv. f_equiv. solve_contractive.
+  Qed.
+
+  Definition valrel_typed := fixpoint valrel_typed_gen.
+
+  Lemma valrel_typed_unfold τ v1 v2 : valrel_typed τ v1 v2 ≡ valrel_typed_gen (fixpoint valrel_typed_gen) τ v1 v2.
+  Proof. do 3 f_equiv. by rewrite -fixpoint_unfold. Qed.
+  Lemma valrel_typed_unfold' τ : valrel_typed τ ≡ valrel_typed_gen (fixpoint valrel_typed_gen) τ.
+  Proof. intros x x'. by rewrite valrel_typed_unfold. Qed.
+  Lemma valrel_typed_unfold'': valrel_typed ≡ valrel_typed_gen (fixpoint valrel_typed_gen).
+  Proof. intros x. by rewrite valrel_typed_unfold'. Qed.
+  Lemma valrel_typed_gen_pre_gen Ψ τ v v' : valrel_typed_gen_pre Ψ τ v v' ≡ valrel_typed_gen Ψ τ v v'.
+  Proof. auto. Qed.
+  Lemma valrel_typed_gen_pre_gen' Ψ τ : valrel_typed_gen_pre Ψ τ ≡ valrel_typed_gen Ψ τ.
+  Proof. intro. intro. auto. Qed.
+
+  Lemma valrel_typed_TUnit_unfold v v' : valrel_typed TUnit v v' ≡ (⌜ v = (()%Vₙₒ : valO) ⌝ ∧ ⌜ v' = (()%Vₙₒ : valO) ⌝)%I.
+  Proof. by rewrite valrel_typed_unfold. Qed.
+  Lemma valrel_typed_TBool_unfold v v' : valrel_typed TBool v v' ≡ (∃ b : bool, ⌜ v = b ⌝ ∧ ⌜ v' = b ⌝)%I.
+  Proof. by rewrite valrel_typed_unfold. Qed.
+  Lemma valrel_typed_TInt_unfold v v' : valrel_typed TInt v v' ≡ (∃ z : Z, ⌜ v = z ⌝ ∧ ⌜ v' = z ⌝)%I.
+  Proof. by rewrite valrel_typed_unfold. Qed.
+  Lemma valrel_typed_TArrow_unfold τ1 τ2 v v' : valrel_typed (TArrow τ1 τ2) v v' ≡ (□ (∀ w w', valrel_typed τ1 w w' -∗ lift NotStuck (valrel_typed τ2) (v w) (v' w')))%I.
+  Proof.
+    rewrite valrel_typed_unfold. rewrite /valrel_typed_gen. simpl.
+    f_equiv. f_equiv. intros w. f_equiv. intro w'. f_equiv.
+    - rewrite valrel_typed_gen_pre_gen. unfold valrel_typed. rewrite -valrel_typed_unfold. auto.
+    - rewrite /lift. f_equiv. simpl. f_equiv. f_equiv. f_equiv. f_equiv.
+      by rewrite valrel_typed_unfold.
+  Qed.
+  Lemma valrel_typed_TSum_unfold τ1 τ2 v v' : valrel_typed (TSum τ1 τ2) v v' ≡ (∃ vi vi', (⌜ v = InjLV vi ⌝ ∧ ⌜ v' = InjLV vi' ⌝ ∧ valrel_typed τ1 vi vi') ∨ (⌜ v = InjRV vi ⌝ ∧ ⌜ v' = InjRV vi' ⌝ ∧ valrel_typed τ2 vi vi'))%I.
+  Proof. rewrite valrel_typed_unfold. simpl. repeat f_equiv; rewrite valrel_typed_gen_pre_gen'; rewrite -valrel_typed_unfold'; auto. Qed.
+  Lemma valrel_typed_TProd_unfold τ1 τ2 v v' : valrel_typed (TProd τ1 τ2) v v' ≡ (∃ v1 v2 v1' v2', ⌜ v = (v1, v2)%Vₙₒ ⌝ ∧ ⌜ v' = (v1' , v2')%Vₙₒ ⌝ ∗ valrel_typed τ1 v1 v1' ∗ valrel_typed τ2 v2 v2')%I.
+  Proof. rewrite valrel_typed_unfold. simpl. repeat f_equiv; rewrite valrel_typed_gen_pre_gen'; rewrite -valrel_typed_unfold'; auto. Qed.
+  Lemma valrel_typed_TRec_unfold τ v v' : valrel_typed (TRec τ) v v' ≡ (∃ w w', ⌜ v = FoldV w ⌝ ∧ ⌜ v' = FoldV w' ⌝ ∧ ▷ (valrel_typed τ.[TRec τ/] w w'))%I.
+  Proof. rewrite valrel_typed_unfold. simpl. repeat f_equiv; rewrite valrel_typed_gen_pre_gen'; rewrite -valrel_typed_unfold'; auto. Qed.
+  Lemma valrel_typed_TVar_unfold X v v' : valrel_typed (TVar X) v v' ≡ False%I.
+  Proof. rewrite valrel_typed_unfold. by simpl. Qed.
+  Lemma valrel_typed_TSTRef_unfold ρ τ v v' :
+    valrel_typed (TSTref ρ τ) v v' ≡
+                 (match ρ with
+                  | TVar X => match Δ !! X with
+                             | Some γ => ∃ i : nat, ⌜ v = i ⌝ ∧ ⌜ v' = i ⌝ ∧
+                                                 inv (nroot .@ γ .@ i) (∃ (w w' : val), i ↪[γ] (w,w') ∗ valrel_typed τ w w')
+                             | None => False
+                             end
+                 | _ => False
+                 end)%I.
+  Proof. rewrite valrel_typed_unfold. simpl. repeat f_equiv. rewrite valrel_typed_gen_pre_gen'; rewrite -valrel_typed_unfold'; auto. Qed.
+  Lemma valrel_typed_TST_unfold ρ τ v v' :
+    valrel_typed (TST ρ τ) v v' ≡
+      (match ρ with
+       | TVar X =>
+         match Δ !! X with
+         | Some γ => ∀ psᵢ : list (prod val val),
+             let vs := psᵢ.*1 in
+             let vs' := psᵢ.*2 in
+             □ (auth_list γ psᵢ -∗
+                          WP v (encode vs) {{ x, ∃ (w w' : val) (psₜ : list (prod val val)),
+                                                auth_list γ psₜ ∧
+                                                let ws := psₜ.*1 in
+                                                let ws' := psₜ.*2 in
+                                                ⌜ x = (encode ws, w)%Vₙₒ ⌝ ∧
+                                                ⌜ rtc lam_step (v' (encode vs')) (encode ws', w')%Vₙₒ ⌝ ∧
+                                                valrel_typed τ w w'
+                                           }}
+               )
+         | None => True
+         end
+       | _ => True
+       end)%I.
+  Proof. rewrite valrel_typed_unfold. simpl. repeat f_equiv. rewrite valrel_typed_gen_pre_gen'; rewrite -valrel_typed_unfold'; auto. Qed.
+
+  Global Instance valrel_typed_persistent τ v v' : Persistent (valrel_typed τ v v').
+  Proof.
+    rewrite /Persistent. revert τ v v'. iLöb as "IHlob". iIntros (τ).
+    iInduction τ as [ | | | τ1 τ2 | τ1 τ2 | τ1 τ2 | τ1 τ2 | τb | ρ τ | ρ τ ] "IH";
+      iIntros (v v'); try by rewrite valrel_typed_unfold; iIntros "#H".
+    - rewrite valrel_typed_TProd_unfold. iIntros "H". iDestruct "H" as (v1 v2 v1' v2') "(-> & -> & H1 & H2)".
+      iExists v1, v2, v1', v2'. repeat iSplit; auto. iApply ("IH" with "H1"). iApply ("IH1" with "H2").
+    - rewrite valrel_typed_TSum_unfold. iIntros "H". iDestruct "H" as (vi vi') "[(-> & -> & H1) | (-> & -> & H2)]"; iExists vi, vi'.
+      + iLeft. repeat iSplit; auto. by iApply ("IH" with "H1").
+      + iRight. repeat iSplit; auto. by iApply ("IH1" with "H2").
+    - rewrite valrel_typed_TRec_unfold. iIntros "H". iDestruct "H" as (w w') "(-> & -> & H)". iExists w, w'. repeat iSplitL ""; auto.
+      iApply bi.later_persistently_1. iNext. by iApply "IHlob".
+    - rewrite valrel_typed_TSTRef_unfold. destruct ρ; auto.
+    - rewrite valrel_typed_TST_unfold. destruct ρ; auto.
+  Qed.
+
+End value_relation.
+
+Section expr_relation.
+
+  Context `{Σ : !gFunctors}.
+  Context `{irisG_inst : !irisG lam_lang Σ}.
+  Context `{ghost_mapG_inst : !ghost_mapG Σ nat (prod val val)}.
+
+  Definition exprel_typed (Δ : list gname) : typeO -n> exprO -n> exprO -n> iPropO Σ := λne τ eᵢ eₛ, lift NotStuck (valrel_typed Δ τ) eᵢ eₛ.
+
+  Definition open_exprel_typed (Γ : list type) (e e' : expr) (τ : type) :=
+    ∀ (Δ : list gname) (vs vs' : list val), big_sepL3 (fun τ v v' => valrel_typed Δ τ v v') Γ vs vs' ⊢
+                                                      exprel_typed Δ τ e.[subst_list_val vs] e'.[subst_list_val vs'].
+
+End expr_relation.
