theories/backtranslations/st_sem/well_defined/logrel/fundamental.v
@@ -1,0 +1,70 @@
+From iris Require Import program_logic.weakestpre.
+From st.lamst Require Import lang types typing.
+From st.lam Require Import lang wkpre generic.lift.
+From st.backtranslations.st_sem Require Import ghost heap expressions.
+From st.backtranslations.st_sem.well_defined.logrel Require Import definition.
+From iris.proofmode Require Import tactics.
+Require Import compat_lemmas.
+
+Section fundamental_theorem.
+
+  Context `{Σ : !gFunctors}.
+  Context `{irisG_inst : !irisG lam_lang Σ}.
+  Context `{ghost_mapG_inst : !ghost_mapG Σ nat (prod val val)}.
+
+  Set Nested Proofs Allowed.
+
+  Lemma fundamental (Γ : list lamst.types.type) (e : lamst.lang.expr) (τ : lamst.types.type)
+        (d : Γ ⊢ₛₜ e : τ) :
+    open_exprel_typed Γ <<e>> <<e>> τ.
+  Proof.
+    induction d; simpl.
+    - admit.
+    - admit.
+    - admit.
+    - admit.
+    - admit.
+    - admit.
+    - admit.
+    - admit.
+    - admit.
+    - admit.
+    - admit.
+    - admit.
+    - admit.
+    - admit.
+    - admit.
+    - admit.
+    - admit.
+    - admit.
+      (* !! intersting ones !! *)
+
+    - (* alloc *)
+      (* cleaning and getting to the gist of it *)
+      iIntros (Δ vs vs') "#Hvsvs'".
+      specialize (IHd Δ vs vs').
+      iDestruct (IHd with "Hvsvs'") as "Hee'". clear IHd. iClear "Hvsvs'".
+      admit.
+    - (* read *)
+      (* cleaning and getting to the gist of it *)
+      iIntros (Δ vs vs') "#Hvsvs'".
+      specialize (IHd Δ vs vs').
+      iDestruct (IHd with "Hvsvs'") as "Hee'". clear IHd. iClear "Hvsvs'".
+      admit.
+    - (* write *)
+      (* cleaning and getting to the gist of it *)
+      iIntros (Δ vs vs') "#Hvsvs'".
+      specialize (IHd1 Δ vs vs').
+      iDestruct (IHd1 with "Hvsvs'") as "Hee'". clear IHd1.
+      specialize (IHd2 Δ vs vs'). clear IHd2.
+      iClear "Hvsvs'".
+      admit.
+    - (* bind *)
+      admit.
+    - (* return *)
+      admit.
+    - (* runst *)
+      admit.
+    - (* equal *)
+      admit.
+
