theories/backtranslations/st_sem/well_defined/logrel/matches_sem.v
@@ -1,0 +1,119 @@
+From iris Require Import program_logic.weakestpre.
+From iris.proofmode Require Import tactics.
+From st.lam Require Import types lang wkpre generic.lift logrel.definitions.
+From st.backtranslations.st_sem Require Import ghost heap.
+From st.backtranslations.st_sem.well_defined.logrel Require Import definition.
+From st Require Import embedding.types.
+From st Require Import prelude.big_op_three.
+
+
+(* Given any non-st type, the two relations agree. *)
+
+Section matches_sem_val.
+
+  Context `{Σ : !gFunctors}.
+  Context `{irisG_inst : !irisG lam_lang Σ}.
+  Context `{ghost_mapG_inst : !ghost_mapG Σ nat (prod val val)}.
+
+  Context (Δ : list gname).
+
+  Notation valrel_sem_typed := (lam.logrel.definitions.valrel_typed NotStuck).
+  Notation valrel_st_typed := (well_defined.logrel.definition.valrel_typed Δ).
+
+  Lemma matches_sem : ∀ (τ : type) (v v' : val) , valrel_sem_typed τ v v' ⊣⊢ valrel_st_typed [|τ|] v v'.
+  Proof.
+    iLöb as "IHlob".
+    iIntros (τ). iInduction τ as [ | | | τ1 τ2 | τ1 τ2 | τ1 τ2 | τb | ] "IH".
+    - setoid_rewrite valrel_typed_TUnit_unfold.
+      setoid_rewrite lam.logrel.definitions.valrel_typed_TUnit_unfold.
+      auto.
+    - setoid_rewrite valrel_typed_TBool_unfold.
+      setoid_rewrite lam.logrel.definitions.valrel_typed_TBool_unfold.
+      auto.
+    - setoid_rewrite valrel_typed_TInt_unfold.
+      setoid_rewrite lam.logrel.definitions.valrel_typed_TInt_unfold.
+      auto.
+    - setoid_rewrite valrel_typed_TProd_unfold. fold embed.
+      setoid_rewrite lam.logrel.definitions.valrel_typed_TProd_unfold.
+      iIntros (v v').
+      iSplit.
+      + iIntros "Hdes". iDestruct "Hdes" as (v1 v2 v1' v2') "(eq1 & eq2 & H1 & H2)".
+        repeat iExists _. repeat iSplit; auto. by iApply "IH". by iApply "IH1".
+      + iIntros "Hdes". iDestruct "Hdes" as (v1 v2 v1' v2') "(eq1 & eq2 & H1 & H2)".
+        repeat iExists _. repeat iSplit; auto. by iApply "IH". by iApply "IH1".
+    - setoid_rewrite valrel_typed_TSum_unfold. fold embed.
+      setoid_rewrite lam.logrel.definitions.valrel_typed_TSum_unfold.
+      iIntros (v v').
+      iSplit.
+      + iIntros "Hdes". iDestruct "Hdes" as (v1 v1') "[(eq1 & eq2 & H) | (eq1 & eq2 & H)]".
+        * repeat iExists _. iLeft. repeat iSplit; eauto. by iApply "IH".
+        * repeat iExists _. iRight. repeat iSplit; eauto. by iApply "IH1".
+      + iIntros "Hdes". iDestruct "Hdes" as (v1 v1') "[(eq1 & eq2 & H) | (eq1 & eq2 & H)]".
+        * repeat iExists _. iLeft. repeat iSplit; eauto. by iApply "IH".
+        * repeat iExists _. iRight. repeat iSplit; eauto. by iApply "IH1".
+    - setoid_rewrite valrel_typed_TArrow_unfold. fold embed.
+      setoid_rewrite lam.logrel.definitions.valrel_typed_TArrow_unfold.
+      iIntros (w w'). iSplit.
+      + iIntros "#H". iModIntro. iIntros (v v') "#H1".
+        iApply (lift_wand _ (valrel_sem_typed τ3)). iIntros (x x') "Hxx'". by iApply "IH1".
+        iApply "H". by iApply "IH".
+      + iIntros "#H". iModIntro. iIntros (v v') "#H1".
+        iApply (lift_wand _ (valrel_st_typed [|τ3|])). iIntros (x x') "Hxx'". by iApply "IH1".
+        iApply "H". by iApply "IH".
+    - setoid_rewrite valrel_typed_TRec_unfold. fold embed.
+      rewrite -embed_TRec_comm.
+      setoid_rewrite lam.logrel.definitions.valrel_typed_TRec_unfold.
+      iIntros (v v'). iSplit.
+      + iIntros "Hdes". iDestruct "Hdes" as (w w') "(eq & eq' & H)".
+        iExists w, w'. repeat iSplit; auto. iNext. by iApply "IHlob".
+      + iIntros "Hdes". iDestruct "Hdes" as (w w') "(eq & eq' & H)".
+        iExists w, w'. repeat iSplit; auto. iNext. by iApply "IHlob".
+    - setoid_rewrite valrel_typed_TVar_unfold.
+      setoid_rewrite lam.logrel.definitions.valrel_typed_TVar_unfold. auto.
+  Qed.
+
+End matches_sem_val.
+
+Section matches_sem_expr.
+
+  Context `{Σ : !gFunctors}.
+  Context `{irisG_inst : !irisG lam_lang Σ}.
+  Context `{ghost_mapG_inst : !ghost_mapG Σ nat (prod val val)}.
+
+  Context (Δ : list gname).
+
+  Notation exprel_sem_typed := (lam.logrel.definitions.exprel_typed NotStuck).
+  Notation exprel_st_typed := (well_defined.logrel.definition.exprel_typed Δ).
+
+  Lemma matches_sem_expr : ∀ (τ : type) (e e' : expr) , exprel_sem_typed τ e e' ⊣⊢ exprel_st_typed [|τ|] e e'.
+  Proof. intros τ e e'. apply lift_equiv. apply matches_sem. Qed.
+
+End matches_sem_expr.
+
+Section matches_sem_expr_open.
+
+  Context `{Σ : !gFunctors}.
+  Context `{irisG_inst : !irisG lam_lang Σ}.
+  Context `{ghost_mapG_inst : !ghost_mapG Σ nat (prod val val)}.
+
+  Notation open_exprel_sem_typed := (lam.logrel.definitions.open_exprel_typed NotStuck).
+  Notation open_exprel_st_typed := (well_defined.logrel.definition.open_exprel_typed).
+
+  Lemma matches_sem_open_expr Γ τ e e' : open_exprel_sem_typed Γ e e' τ <-> open_exprel_st_typed (embed <$> Γ) e e' [|τ|].
+  Proof.
+    split.
+    - intro Hsem. iIntros (Δ vs vs') "Hvsvs'".
+      iApply matches_sem_expr.
+      iApply Hsem.
+      iApply (big_sepL3_impl with "[Hvsvs']").
+      iApply (big_sepL3_fmap_l with "Hvsvs'").
+      iModIntro. iIntros (τ' v v') "H". by iApply matches_sem.
+    - intro Hsem. iIntros (vs vs') "Hvsvs'".
+      iApply (matches_sem_expr []).
+      iApply Hsem.
+      iApply (big_sepL3_fmap_l).
+      iApply (big_sepL3_impl with "Hvsvs'").
+      iModIntro. iIntros (τ' v v') "H". by iApply matches_sem.
+  Qed.
+
+End matches_sem_expr_open.
